theories/tl_borrow.v
@@ -1,0 +1,50 @@
+From lrust Require Export lifetime.
+From iris.base_logic.lib Require Export thread_local.
+From iris.proofmode Require Import tactics.
+
+Definition tl_borrow `{invG Σ, lifetimeG Σ, thread_localG Σ}
+           (κ : lifetime) (tid : thread_id) (N : namespace) (P : iProp Σ) :=
+  (∃ i, idx_borrow κ i P ∗ tl_inv tid N (idx_borrow_own 1 i))%I.
+
+Notation "&tl{ κ | tid | N } P" := (tl_borrow κ tid N P)
+  (format "&tl{ κ | tid | N } P", at level 20, right associativity) : uPred_scope.
+
+Section tl_borrow.
+  Context `{invG Σ, lifetimeG Σ, thread_localG Σ}
+          (tid : thread_id) (N : namespace) (P : iProp Σ).
+
+  Global Instance tl_borrow_persistent κ : PersistentP (&tl{κ|tid|N} P) := _.
+  Global Instance tl_borrow_proper κ :
+    Proper ((⊣⊢) ==> (⊣⊢)) (tl_borrow κ tid N).
+  Proof.
+    intros P1 P2 EQ. apply uPred.exist_proper. intros i. by rewrite EQ.
+  Qed.
+
+  Lemma borrow_tl κ `(nclose lftN ⊆ E): &{κ}P ={E}=∗ &tl{κ|tid|N}P.
+  Proof.
+    iIntros "HP". unfold borrow. iDestruct "HP" as (i) "[#? Hown]".
+    iExists i. iFrame "#". iApply (tl_inv_alloc tid E N with "[Hown]"). auto.
+  Qed.
+
+  Lemma tl_borrow_acc q κ E F :
+    nclose lftN ⊆ E → nclose tlN ⊆ E → nclose N ⊆ F →
+    &tl{κ|tid|N}P ⊢ q.[κ] ∗ tl_own tid F ={E}=∗ ▷P ∗ tl_own tid (F ∖ N) ∗
+                     (▷P ∗ tl_own tid (F ∖ N) ={E}=∗ q.[κ] ∗ tl_own tid F).
+  Proof.
+    iIntros (???) "#HP[Hκ Htlown]".
+    iDestruct "HP" as (i) "(#Hpers&#Hinv)".
+    iMod (tl_inv_open with "Hinv Htlown") as "(>Hown&Htlown&Hclose)"; try done.
+    iMod (idx_borrow_acc with "Hpers [$Hown $Hκ]") as "[HP Hclose']". done.
+    iIntros "{$HP $Htlown}!>[HP Htlown]".
+    iMod ("Hclose'" with "HP") as "[Hown $]". iApply "Hclose". by iFrame.
+  Qed.
+
+  Lemma tl_borrow_shorten κ κ': κ ⊑ κ' ⊢ &tl{κ'|tid|N}P -∗ &tl{κ|tid|N}P.
+  Proof.
+    iIntros "Hκκ' H". iDestruct "H" as (i) "[??]". iExists i. iFrame.
+    iApply (idx_borrow_shorten with "Hκκ' H").
+  Qed.
+
+End tl_borrow.
+
+Typeclasses Opaque tl_borrow.
